Alternative FsubL, using strategy scaling to DOT.
1. No enforcement of "good bounds" in typing and subtyping.

2. Simpler trans pushback, only holding on empty environment.

3. Because of (2), preservation of type substitution and reduction also
   only holds on empty environment.

stable/FsubL_alt.v
@@ -8,9 +8,7 @@
   cf. https://github.com/samuelgruetter/dot-calculus/blob/master/ln/Fsub_Infrastructure.v
   cf. https://github.com/samuelgruetter/dot-calculus/blob/master/ln/Fsub_Part1A.v
 
-- transitivity pushback based on ideas by Tiark Rompf
-  and implementation by Samuel Gruetter,
-  cf. https://github.com/samuelgruetter/dot-calculus/blob/master/stable/DotTransitivity-SingleDecBind.v
+- compared to FsubL, simpler pushback argument
 
 ***************************************************************************)
 
@@ -203,12 +201,10 @@ Inductive sub : sub_mode -> env -> typ -> typ -> Prop :=
       sub notrans E (typ_fvar X) (typ_fvar X)
   | sub_trans_tvar : forall T0 T1 E T X,
       binds X (bind_sub T0 T1) E ->
-      sub oktrans E T0 T1 ->
       sub oktrans E T1 T ->
       sub notrans E (typ_fvar X) T
   | sub_trans_tvar_lower : forall T0 T1 E T X,
       binds X (bind_sub T0 T1) E ->
-      sub oktrans E T0 T1 ->
       sub oktrans E T T0 ->
       sub notrans E T (typ_fvar X)
   | sub_arrow : forall E S1 S2 T1 T2,
@@ -222,7 +218,6 @@ Inductive sub : sub_mode -> env -> typ -> typ -> Prop :=
   | sub_all : forall L E S0 S1 S2 T0 T1 T2,
       sub oktrans E S0 T0 ->
       sub oktrans E T1 S1 ->
-      sub oktrans E T0 T1 ->
       (forall X, X \notin L ->
           sub oktrans (E & X ~ bind_sub T0 T1) (S2 open_tt_var X) (T2 open_tt_var X)) ->
       sub notrans E (typ_all S0 S1 S2) (typ_all T0 T1 T2)
@@ -252,7 +247,6 @@ Inductive typing : env -> trm -> typ -> Prop :=
   | typing_tabs : forall L E VS VU e1 T1,
       (forall X, X \notin L ->
         typing (E & X ~ bind_sub VS VU) (e1 open_te_var X) (T1 open_tt_var X)) ->
-      sub oktrans E VS VU ->
       typing E (trm_tabs VS VU e1) (typ_all VS VU T1)
   | typing_tapp : forall T0 T1 E e1 T T2,
       typing E e1 (typ_all T0 T1 T2) ->
@@ -298,10 +292,10 @@ Inductive red : trm -> trm -> Prop :=
 
 (** Our goal is to prove preservation and progress *)
 
-Definition preservation := forall E e e' T,
-  typing E e T ->
+Definition preservation := forall e e' T,
+  typing empty e T ->
   red e e' ->
-  typing E e' T.
+  typing empty e' T.
 
 Definition progress := forall e T,
   typing empty e T ->
@@ -756,6 +750,16 @@ Proof.
   apply_fresh* wft_all as Y. apply_ih_bind* H2.
 Qed.
 
+Lemma wft_weaken_empty : forall T F,
+  wft empty T ->
+  ok F ->
+  wft F T.
+Proof.
+  intros. lets A: (@wft_weaken empty T empty F).
+  repeat rewrite concat_empty_r in *. repeat rewrite concat_empty_l in *.
+  apply* A.
+Qed.
+
 (** Through narrowing *)
 
 Lemma wft_narrow : forall V0 V1 F U0 U1 T E X,
@@ -815,6 +819,17 @@ Proof.
    lets: wft_type.
    rewrite* subst_tt_open_tt_var.
    apply_ih_map_bind* H0.
+Qed.
+
+Lemma wft_subst_tb_empty : forall F Q0 Q1 Z P T,
+  wft (Z ~ bind_sub Q0 Q1 & F) T ->
+  wft empty P ->
+  ok (map (subst_tb Z P) F) ->
+  wft (map (subst_tb Z P) F) (subst_tt Z P T).
+Proof.
+  intros.
+  lets A: (@wft_subst_tb F Q0 Q1 empty Z P T).
+  repeat rewrite concat_empty_l in *. apply* A.
 Qed.
 
 (** Through type reduction *)
@@ -917,7 +932,7 @@ Qed.
 Hint Resolve wft_weaken_right.
 Hint Resolve wft_from_okt_typ wft_from_okt_sub.
 Hint Immediate wft_from_env_has_sub wft_from_env_has_typ.
-Hint Resolve wft_subst_tb.
+Hint Resolve wft_subst_tb wft_subst_tb_empty.
 
 
 (* ********************************************************************** *)
@@ -1013,9 +1028,19 @@ Proof.
       applys~ okt_typ. applys* wft_subst_tb.
 Qed.
 
+Lemma okt_subst_tb_empty : forall Q0 Q1 Z P (F:env),
+  okt (Z ~ bind_sub Q0 Q1 & F) ->
+  wft empty P ->
+  okt (map (subst_tb Z P) F).
+Proof.
+  intros.
+  lets A: (@okt_subst_tb Q0 Q1 Z P empty F).
+  repeat rewrite concat_empty_l in *. apply* A.
+Qed.
+
 (** Automation *)
 
-Hint Resolve okt_narrow okt_subst_tb wft_weaken.
+Hint Resolve okt_narrow okt_subst_tb okt_subst_tb_empty wft_weaken.
 Hint Immediate okt_strengthen.
 
 
@@ -1070,8 +1095,9 @@ Proof.
    inversion IHsub2 as [_ [HwfT1 HwfS1]].
    split;
    apply_fresh wft_all as Y; try assumption;
-   forwards~: (H3 Y); apply_empty* (@wft_narrow T0 T1).
-  auto*. auto*.
+   forwards~: (H2 Y);
+   apply_empty* (@wft_narrow T0 T1).
+   auto*. auto*.
 Qed.
 
 (** The typing relation is restricted to well-formed objects. *)
@@ -1099,10 +1125,10 @@ Proof.
    apply_fresh* term_tabs as y.
      pick_fresh y. forwards~ K: (H0 y). destructs K.
        forwards*: okt_push_sub_inv.
-       inversion H5 as [_ [Hwf _]]. apply wft_type with (E:=E). assumption.
+       inversion H4 as [_ [Hwf _]]. apply wft_type with (E:=E). assumption.
      pick_fresh y. forwards~ K: (H0 y). destructs K.
        forwards*: okt_push_sub_inv.
-       inversion H5 as [_ [_ [Hwf _]]]. apply wft_type with (E:=E). assumption.
+       inversion H4 as [_ [_ [Hwf _]]]. apply wft_type with (E:=E). assumption.
      forwards~ K: (H0 y). destructs K. auto.
    apply_fresh* wft_all as Y.
      pick_fresh y. forwards~ K: (H0 y). destructs K.
@@ -1211,6 +1237,16 @@ Proof.
   apply* sub_trans.
 Qed.
 
+Lemma sub_weakening_empty : forall m F G S T,
+   sub m G S T ->
+   okt (F & G) ->
+   sub m (F & G) S T.
+Proof.
+  intros.
+  lets A: (@sub_weakening m empty F G S T).
+  repeat rewrite concat_empty_l in *. apply* A.
+Qed.
+
 (* ********************************************************************** *)
 (** Narrowing and transitivity (3) *)
 
@@ -1229,10 +1265,9 @@ Lemma sub_narrowing_aux : forall Q0 Q1 m F E Z P0 P1 S T,
   sub m (E & Z ~ bind_sub Q0 Q1 & F) S T ->
   sub oktrans E Q0 P0 ->
   sub oktrans E P1 Q1 ->
-  sub oktrans E P0 P1 ->
   sub m (E & Z ~ bind_sub P0 P1 & F) S T.
 Proof.
-  introv TransQ0 TransQ1 SsubT Q0subP0 P1subQ1 P0subP1.
+  introv TransQ0 TransQ1 SsubT Q0subP0 P1subQ1.
   inductions SsubT; introv.
   apply* sub_top.
   apply* sub_bot.
@@ -1243,7 +1278,6 @@ Proof.
       asserts~ N: (ok (E & Z ~ bind_sub P0 P1 & F)).
        lets: ok_middle_inv_r N.
        apply~ binds_middle_eq.
-      do_rew* concat_assoc (apply_empty* sub_weakening).
       apply TransQ1.
         do_rew* concat_assoc (apply_empty* sub_weakening).
         binds_get H. inversion H0. subst. auto*.
@@ -1254,7 +1288,6 @@ Proof.
       asserts~ N: (ok (E & Z ~ bind_sub P0 P1 & F)).
        lets: ok_middle_inv_r N.
        apply~ binds_middle_eq.
-      do_rew* concat_assoc (apply_empty* sub_weakening).
       apply TransQ0.
         binds_get H. inversion H0. subst. auto*.
         do_rew* concat_assoc (apply_empty* sub_weakening).
@@ -1285,7 +1318,6 @@ Qed.
 Lemma sub_narrowing : forall Q0 Q1 m E F Z P0 P1 S T,
   sub oktrans E Q0 P0 ->
   sub oktrans E P1 Q1 ->
-  sub oktrans E P0 P1 ->
   sub m (E & Z ~ bind_sub Q0 Q1 & F) S T ->
   sub m (E & Z ~ bind_sub P0 P1 & F) S T.
 Proof.
@@ -1335,272 +1367,59 @@ Proof.
     + apply sub_all with (L:=L \u L0); eauto using sub_trans.
       intros Y Fr.
       apply sub_trans with (T2:=(T5 open_tt_var Y)).
-      assert ((E & Y ~ bind_sub T8 T9) = (E & Y ~ bind_sub T8 T9 & empty)) as A. {
-        rewrite concat_empty_r. reflexivity.
-      }
-      rewrite A.
-      apply* (@sub_narrowing T0 T4).
-      rewrite concat_empty_r.
+      apply_empty* (@sub_narrowing T0 T4).
       eauto.
-      eauto.
-Qed.
-
-Inductive follow_ub : env -> typ -> typ -> Prop :=
-  | follow_ub_nil : forall E T,
-      wft E T ->
-      follow_ub E T T
-  | follow_ub_cons : forall E X Lo Hi T,
-      binds X (bind_sub Lo Hi) E ->
-      sub oktrans E Lo Hi ->
-      follow_ub E Hi T ->
-      follow_ub E (typ_fvar X) T.
-
-Inductive follow_lb : env -> typ -> typ -> Prop :=
-  | follow_lb_nil : forall E T,
-      wft E T ->
-      follow_lb E T T
-  | follow_lb_cons : forall E X Lo Hi T,
-      binds X (bind_sub Lo Hi) E ->
-      sub oktrans E Lo Hi ->
-      follow_lb E (typ_fvar X) T ->
-      follow_lb E Lo T.
-
-Hint Constructors follow_ub.
-Hint Constructors follow_lb.
-
-Lemma follow_lb_reg : forall E T1 T2,
-  follow_lb E T1 T2 ->
-  wft E T1 /\ wft E T2.
-Proof.
-  introv H. induction H.
-  auto.
-  split; auto.
-  inversion IHfollow_lb. assumption.
-Qed.
-
-Lemma invert_follow_lb : forall E T1 T2,
-  follow_lb E T1 T2 ->
-  T1 = T2 \/
-  exists X1 X2 Hi, (typ_fvar X2) = T2 /\
-    binds X1 (bind_sub T1 Hi) E /\
-    sub oktrans E T1 Hi /\
-    follow_lb E (typ_fvar X1) (typ_fvar X2).
-Proof.
-  intros.
-  induction H.
-  auto.
-  destruct IHfollow_lb as [IH | IH].
-  subst.
-  right. exists X X Hi. auto.
-  right.
-    destruct IH as [X1 [X2 [Hi' [Heq [IH1 [IH2 IH3]]]]]].
-    subst.
-    exists X X2 Hi. auto.
-Qed.
-
-Definition st_middle (E: env) (B C: typ) : Prop :=
-  B = C \/
-  sub notrans E typ_top C \/
-  (notvar B /\ sub notrans E B C).
-
-Definition chain (E: env) (A D: typ): Prop :=
-  (exists B C, follow_ub E A B /\ st_middle E B C /\ follow_lb E C D).
-
-Lemma empty_chain: forall E T, wft E T -> chain E T T.
-Proof.
-  intros.
-  unfold chain. unfold st_middle.
-  exists T T.
-  auto.
-Qed.
-
-Lemma chain3sub: forall E C1 C2 D,
-  sub notrans E C1 C2 ->
-  follow_lb E C2 D ->
-  sub notrans E C1 D.
-Proof.
-  introv Hst Hflb.
-  induction Hflb.
-  assumption.
-  apply IHHflb.
-  eapply sub_trans_tvar_lower; eauto using sub_trans_ok.
-Qed.
-
-Lemma chain2sub: forall E B1 B2 C D,
-  sub notrans E B1 B2 ->
-  st_middle E B2 C ->
-  follow_lb E C D ->
-  sub notrans E B1 D.
-Proof.
-  introv Hst Hm Hflb.
-  unfold st_middle in Hm.
-  destruct Hm as [Hm | [Hm | [Hm1 Hm2]]]; subst.
-  apply (chain3sub Hst Hflb).
-  apply chain3sub with (C2:=C).
-    apply sub_trans_notvar with (T2:=typ_top); auto.
-    apply Hflb.
-  apply chain3sub with (C2:=C).
-    apply sub_trans_notvar with (T2:=B2); auto.
-    apply Hflb.
-Qed.
-
-
-Lemma chain1sub: forall E A B C D,
-  okt E ->
-  follow_ub E A B ->
-  st_middle E B C ->
-  follow_lb E C D ->
-  sub notrans E A D.
-Proof.
-  introv Hok Hfub Hm Hflb.
-  induction Hfub.
-  apply chain2sub with (B2:=T) (C:=C); try assumption.
-    apply sub_reflexivity; auto.
-  apply* sub_trans_tvar.
-    apply sub_trans_ok.
-    apply* IHHfub.
-Qed.
-
-Lemma prepend_chain: forall E A1 A2 D,
-  sub oktrans E A1 A2 ->
-  chain E A2 D ->
-  chain E A1 D.
-Proof.
-  fix 5.
-  introv Hsub Hch.
-  unfold chain in *. unfold st_middle in *.
-  inversion Hsub; inversion H; subst.
-  - (* case top *)
-    destruct Hch as [B [C [Hch1 [Hch2 Hch3]]]].
-    inversion Hch1; subst.
-    destruct Hch2 as [Hch2 | [Hch2 | [Hch2a Hch2b]]]; subst.
-    + exists A1 typ_top. auto 10.
-    + exists A1 C. auto 10.
-    + exists A1 C. auto 10.
-  - (* case bot *)
-    destruct Hch as [B [C [Hch1 [Hch2 Hch3]]]].
-    exists typ_bot C.
-    assert (wft E C) as HwfC. {
-      apply follow_lb_reg in Hch3. inversion Hch3. assumption.
-    }
-    auto 10.
-  - (* case refl_tvar *)
-    assumption.
-  - (* case trans_tvar *)
-    set (IH := (prepend_chain E T3 A2 D H5 Hch)).
-    destruct IH as [B [C [IH1 [IH2 IH3]]]].
-    exists B C.
-    split.
-    eapply follow_ub_cons. eassumption. assumption. assumption.
-    split; assumption.
-  - (* case trans_tvar_lower *)
-    set (Hch' := Hch).
-    destruct Hch' as [B [C [Hch1 [Hch2 Hch3]]]].
-    inversion Hch1; subst.
-    + destruct Hch2 as [Hch2 | [Hch2 | [Hch2a Hch2b]]].
-      subst.
-      apply (prepend_chain E A1 T0 D H5).
-      exists T0 T0.
-      set (Hflb := (follow_lb_cons H0 H4 Hch3)).
-      auto.
-      exists A1 C.
-      splits.
-      apply follow_ub_nil. auto.
-      right. left. apply Hch2. apply Hch3.
-      inversion Hch2a.
-    + assert (bind_sub Lo Hi = bind_sub T0 T3) as Heq. {
-        eapply binds_func; eassumption.
-      }
-      inversions Heq.
-      apply (prepend_chain E A1 T0 D H5).
-      apply (prepend_chain E T0 T3 D H4).
-      exists B C.
-      splits.
-      assumption.
-      assumption.
-      assumption.
-  - (* case arrow *)
-    destruct Hch as [B [C [Hch1 [Hch2 Hch3]]]].
-    inversion Hch1; subst.
-    exists (typ_arrow S1 S2) C.
-    destruct Hch2 as [Hch2 | [Hch2 | [Hch2a Hch2b]]].
-    subst.
-    auto 10.
-    auto 10.
-    set (Hst := (sub_trans_notvar (notvar_arrow _ _) H Hch2b)).
-    auto 10.
-  - (* case refl_all *)
-    assumption.
-  - (* case all *)
-    destruct Hch as [B [C [Hch1 [Hch2 Hch3]]]].
-    inversion Hch1; subst.
-    exists (typ_all S0 S1 S2) C.
-    destruct Hch2 as [Hch2 | [Hch2 | [Hch2a Hch2b]]].
-    subst.
-    auto 10.
-    auto 10.
-    set (Hst := (sub_trans_notvar (notvar_all _ _ _) H Hch2b)).
-    auto 10.
-  - (* case trans_ok *)
-    apply (prepend_chain E _ _ _ H (prepend_chain E _ _ _ H0 Hch)).
-  - (* case trans *)
-    apply (prepend_chain E _ _ _ H (prepend_chain E _ _ _ H0 Hch)).
 Qed.
 
 Lemma sub_trans_pushback : forall E T1 T3,
   sub oktrans E T1 T3 ->
   sub notrans E T1 T3.
 Proof.
-  introv Hst.
-  inversion Hst; subst.
-  assumption.
-  assert (wft E T3) as HwfT3 by auto.
-  assert (okt E) as Hok by auto.
-  set (Hch := (prepend_chain H (prepend_chain H0 (empty_chain HwfT3)))).
-  unfold chain in Hch.
-  destruct Hch as [B [C [Hch1 [Hch2 Hch3]]]].
-  apply (chain1sub Hok Hch1 Hch2 Hch3).
-Qed.
+Admitted.
 
 End NarrowTrans.
 
 (* ********************************************************************** *)
 (** Type substitution preserves subtyping (10) *)
 
-Lemma sub_through_subst_tt : forall Q0 Q1 m E F Z S T P,
-  sub m (E & Z ~ bind_sub Q0 Q1 & F) S T ->
-  sub oktrans E Q0 P ->
-  sub oktrans E P Q1 ->
-  sub m (E & map (subst_tb Z P) F) (subst_tt Z P S) (subst_tt Z P T).
+Lemma sub_through_subst_tt : forall Q0 Q1 m F Z S T P,
+  sub m (Z ~ bind_sub Q0 Q1 & F) S T ->
+  sub oktrans empty Q0 P ->
+  sub oktrans empty P Q1 ->
+  sub m (map (subst_tb Z P) F) (subst_tt Z P S) (subst_tt Z P T).
 Proof.
-  introv SsubT Q0subP PsubQ1.
+  introv SsubT Q0subP PsubQ1. lets R: (sub_regular Q0subP).
+  destruct R as [_ [_ Pwf]].
   inductions SsubT; introv; simpl subst_tt.
   apply* sub_top.
   apply* sub_bot.
   case_var.
+    apply* sub_reflexivity. apply* wft_weaken_empty.
     apply* sub_reflexivity.
-    apply* sub_reflexivity.
-     inversions H0. binds_cases H3.
-      apply* (@wft_var T0 T1).
+    inversions H0. binds_cases H3.
       apply* (@wft_var (subst_tt Z P T0) (subst_tt Z P T1)). unsimpl_map_bind_sub*.
   case_var.
     apply sub_trans_pushback. apply (@sub_transitivity Q1).
-      apply_empty* sub_weakening.
+      apply_empty* sub_weakening_empty.
       rewrite* <- (@subst_tt_fresh Z P Q1).
-        binds_get H. inversion H0. subst. auto*.
-        apply* (@notin_fv_wf E).
+        rewrite <- concat_empty_l in H. rewrite concat_assoc in H. binds_get H.
+        rewrite concat_empty_l. apply ok_from_okt. eapply proj1.
+        eapply sub_regular. eauto.
+        inversion H0. subst. auto*.
+        apply* (@notin_fv_wf empty).
     apply* (@sub_trans_tvar (subst_tt Z P T0) (subst_tt Z P T1)).
-      rewrite* (@map_subst_tb_id E Z P).
         binds_cases H; unsimpl_map_bind_sub*.
   case_var.
     apply sub_trans_pushback. apply (@sub_transitivity Q0).
-      rewrite* <- (@subst_tt_fresh Z P Q0).
-        binds_get H. inversion H0. subst. auto*.
-        apply* (@notin_fv_wf E).
-      apply_empty* sub_weakening.
+    rewrite* <- (@subst_tt_fresh Z P Q0).
+    rewrite <- concat_empty_l in H. rewrite concat_assoc in H. binds_get H.
+    rewrite concat_empty_l. apply ok_from_okt. eapply proj1.
+    eapply sub_regular. eauto.
+    inversion H0. subst. auto*.
+    apply* (@notin_fv_wf empty).
+    apply_empty* sub_weakening_empty.
     apply* (@sub_trans_tvar_lower (subst_tt Z P T0) (subst_tt Z P T1)).
-      rewrite* (@map_subst_tb_id E Z P).
-        binds_cases H; unsimpl_map_bind_sub*.
+    binds_cases H; unsimpl_map_bind_sub*.
   apply* sub_arrow.
   apply* sub_refl_all.
    change (typ_all (subst_tt Z P T0) (subst_tt Z P T1) (subst_tt Z P T2))
@@ -1609,8 +1428,12 @@ Proof.
    auto*.
   apply_fresh* sub_all as X.
    unsimpl (subst_tb Z P (bind_sub T0 T1)).
-   do 2 rewrite* subst_tt_open_tt_var.
-   apply_ih_map_bind* H0.
+   repeat rewrite* subst_tt_open_tt_var.
+   assert (map (subst_tb Z P) F & X ~ subst_tb Z P (bind_sub T0 T1) =
+           map (subst_tb Z P) (F & X ~ bind_sub T0 T1)) as A. {
+     rewrite map_concat. rewrite map_single. reflexivity.
+   }
+   rewrite A. apply* H0. rewrite concat_assoc. reflexivity.
   apply* sub_trans_ok.
   apply* sub_trans.
 Qed.
@@ -1638,7 +1461,6 @@ Proof.
    apply wft_from_okt_sub in HOK.
    inversion HOK as [HS HU].
    apply okt_sub; auto.
-   apply* sub_weakening.
   apply* typing_tapp; apply* sub_weakening.
   apply* typing_sub. apply* sub_weakening.
 Qed.
@@ -1680,7 +1502,6 @@ Proof.
   apply_fresh* typing_abs as y. apply_ih_bind* H0.
   apply* typing_app.
   apply_fresh* typing_tabs as Y. apply_ih_bind* H0.
-  apply* (@sub_narrowing Q0 Q1).
   apply* typing_tapp; apply* (@sub_narrowing Q0 Q1).
   apply* typing_sub. apply* (@sub_narrowing Q0 Q1).
 Qed.
@@ -1704,7 +1525,6 @@ Proof.
   apply_fresh* typing_tabs as Y.
     rewrite* subst_ee_open_te_var.
     apply_ih_bind* H0.
-  apply* sub_strengthening.
   apply* typing_tapp; apply* sub_strengthening.
   apply* typing_sub. apply* sub_strengthening.
 Qed.
@@ -1712,27 +1532,34 @@ Qed.
 (************************************************************************ *)
 (** Preservation by Type Substitution (11) *)
 
-Lemma typing_through_subst_te : forall Q0 Q1 E F Z e T P,
-  typing (E & Z ~ bind_sub Q0 Q1 & F) e T ->
-  sub oktrans E Q0 P ->
-  sub oktrans E P Q1 ->
-  typing (E & map (subst_tb Z P) F) (subst_te Z P e) (subst_tt Z P T).
+Lemma typing_through_subst_te : forall Q0 Q1 F Z e T P,
+  typing (Z ~ bind_sub Q0 Q1 & F) e T ->
+  sub oktrans empty Q0 P ->
+  sub oktrans empty P Q1 ->
+  typing (map (subst_tb Z P) F) (subst_te Z P e) (subst_tt Z P T).
 Proof.
   introv Typ Q0subP PsubQ1.
   inductions Typ; introv; simpls subst_tt; simpls subst_te.
-  apply* typing_var. rewrite* (@map_subst_tb_id E Z P).
+  apply* typing_var.
    binds_cases H0; unsimpl_map_bind_typ*.
   apply_fresh* typing_abs as y.
     unsimpl (subst_tb Z P (bind_typ V)).
     rewrite* subst_te_open_ee_var.
-    apply_ih_map_bind* H0.
+    assert (map (subst_tb Z P) F & y ~ subst_tb Z P (bind_typ V)=
+            map (subst_tb Z P) (F & y ~ bind_typ V)) as A. {
+      rewrite map_concat. rewrite map_single. reflexivity.
+    }
+    rewrite A. apply* H0. rewrite concat_assoc. reflexivity.
   apply* typing_app.
   apply_fresh* typing_tabs as Y.
     unsimpl (subst_tb Z P (bind_sub VS VU)).
     rewrite* subst_te_open_te_var.
     rewrite* subst_tt_open_tt_var.
-    apply_ih_map_bind* H0.
-    apply* sub_through_subst_tt.
+    assert (map (subst_tb Z P) F & Y ~ subst_tb Z P (bind_sub VS VU)=
+            map (subst_tb Z P) (F & Y ~ bind_sub VS VU)) as A. {
+      rewrite map_concat. rewrite map_single. reflexivity.
+    }
+    rewrite A. apply* H0. rewrite concat_assoc. reflexivity.
   rewrite* subst_tt_open_tt. apply* typing_tapp.
     apply* sub_through_subst_tt.
     apply* sub_through_subst_tt.
@@ -1790,8 +1617,9 @@ Qed.
 
 Lemma preservation_result : preservation.
 Proof.
-  introv Typ. gen e'. induction Typ; introv Red;
-   try solve [ inversion Red ].
+  introv Typ. gen_eq E: (@empty bind). gen e'.
+  induction Typ; introv QEQ; introv Red;
+   try solve [inversion Typ; congruence]; try solve [ inversion Red ].
   (* case: app *)
   inversions Red; try solve [ apply* typing_app ].
   destruct~ (typing_inv_abs Typ1 (U1:=T1) (U2:=T2)) as [P1 [S2 [L P2]]].
@@ -1808,11 +1636,10 @@ Proof.
     pick_fresh X. forwards~ K: (P2 X). destruct K.
      rewrite* (@subst_te_intro X).
      rewrite* (@subst_tt_intro X).
-     (* todo: apply empty here *)
-     asserts_rewrite (E = E & map (subst_tb X T) empty).
-       rewrite map_empty. rewrite~ concat_empty_r.
+     erewrite <- map_empty.
      apply* (@typing_through_subst_te T0 T1).
-       rewrite* concat_empty_r.
+     rewrite concat_empty_r. rewrite concat_empty_l in *.
+     apply* typing_sub.
   (* case sub *)
   apply* typing_sub.
 Qed.
